ulib/FStar.Set.fsti
@@ -40,6 +40,7 @@ val singleton (#a:eqtype) (x:a)
 val union      : #a:eqtype -> set a -> set a -> Tot (set a)
 val intersect  : #a:eqtype -> set a -> set a -> Tot (set a)
 val complement : #a:eqtype -> set a -> Tot (set a)
+val intension  : #a:eqtype -> (a -> bool) -> GTot (set a)
 
 (* a property about sets *)
 let disjoint (#a:eqtype) (s1: set a) (s2: set a) =
@@ -74,6 +75,10 @@ val mem_complement: #a:eqtype -> x:a -> s:set a -> Lemma
    (requires True)
    (ensures (mem x (complement s) = not (mem x s)))
    [SMTPat (mem x (complement s))]
+
+val mem_intension: #a:eqtype -> x:a -> f:(a -> bool) -> Lemma
+  (requires True)
+  (ensures (mem x (intension f) = f x))
 
 val mem_subset: #a:eqtype -> s1:set a -> s2:set a -> Lemma
    (requires (forall x. mem x s1 ==> mem x s2))
